Validator/StateSetFormalism/Horn.lean
@@ -1,18 +1,15 @@
 import Validator.StateSetFormalism.Formula
 
-namespace Validator
-open Formula
+namespace Validator.Formula
 
 abbrev Clause.IsHorn {n} (γ : Clause n) : Prop :=
   γ.countP Prod.snd ≤ 1
 
-namespace Formula.CNF
-
-def ofPartialModel {n} {V : VarSet' n} (M : PartialModel V) : CNF n :=
-  V.val.mapFinIdx fun i var h ↦ [(var, M[i])]
+def Cube.ofPartialModel {n} {V : VarSet' n} (M : PartialModel V) : Cube n :=
+  V.val.mapFinIdx fun i var h ↦ (var, M[i])
 
 @[simp]
-lemma models_ofPartialModel {n} {V : VarSet' n} {M : PartialModel V} :
+lemma Cube.models_ofPartialModel {n} {V : VarSet' n} {M : PartialModel V} :
   models (ofPartialModel M) = M.models := by
     ext M'
     simp only [ofPartialModel, mem_models, List.mem_mapFinIdx, Literal.mem_models,
@@ -23,27 +20,85 @@ lemma models_ofPartialModel {n} {V : VarSet' n} {M : PartialModel V} :
       specialize h ⟨i, hi⟩
       simp_all
 
+namespace CNF
+
+-- write in terms of filterMap?
+def propagate_literal {n} (φ : CNF n) (l : Literal n) : CNF n :=
+  (φ.filter fun γ ↦ not (γ.contains l)).map (List.filter (· ≠ l.negate))
+
+lemma length_propagate_literal {n} {φ : CNF n} {l} : (φ.propagate_literal l).length ≤ φ.length :=
+  by
+    simp only [propagate_literal, List.length_map]
+    apply List.length_filter_le
+
+lemma IsHorn_propagate_literal {n} {φ : CNF n} {l} :
+  φ.Forall Clause.IsHorn → (φ.propagate_literal l).Forall Clause.IsHorn :=
+  by
+    simp only [List.forall_iff_forall_mem, Clause.IsHorn, List.countP_eq_length_filter,
+      propagate_literal, List.mem_map, List.mem_filter, forall_exists_index, and_imp]
+    intro h1 γ' γ hγ h3 rfl
+    rw [List.filter_comm]
+    grind only [List.length_filter_le]
+
+lemma vars_propagate_literal {n} {φ : CNF n} {l} : (φ.propagate_literal l).vars ⊆ φ.vars \ {l.1} :=
+  by
+    intro v hv
+    simp [vars, propagate_literal, Literal.negate] at hv
+    simp [vars]
+    grind
+
 def rename {n} (φ : CNF n) (vars vars' : VarSet' n)
   (h1 : vars.val.length = vars'.val.length) : CNF n :=
   sorry
 
 end Formula.CNF
+open Formula
 
 structure Horn n where
 
   vars : VarSet' n
 
-  formula : CNF n
+  empty : Bool
 
-  prop : formula.Forall Clause.IsHorn
+  unit_literals : Cube n
 
-  subset_vars : ∀ i ∈ formula.vars, i ∈ vars.val
+  clauses : CNF n
+
+  horn_prop : clauses.Forall Clause.IsHorn
+
+  clauses_prop : clauses.Forall fun γ ↦ 2 ≤ γ.length
+
+  subset_vars : ∀ i ∈ unit_literals.vars ∪ clauses.vars, i ∈ vars.val
 
   deriving DecidableEq, Repr
 
 namespace Horn
 
-abbrev models {n} (φ : Horn n) : Models n := φ.formula.models
+def toCNF {n} (φ : Horn n) : CNF n :=
+    if φ.empty then
+      [[]]
+    else
+      φ.unit_literals.map (fun l ↦ [l]) ++ φ.clauses
+
+abbrev models {n} (φ : Horn n) : Models n := φ.toCNF.models
+
+lemma models_eq {n} {φ : Horn n} :
+  φ.models = if φ.empty then ∅ else φ.unit_literals.models ∩ φ.clauses.models :=
+  by
+    simp only [models, toCNF]
+    split
+    · simp [CNF.models]
+    · ext M
+      simp only [CNF.mem_models, List.mem_append, List.mem_map,
+        Set.mem_inter_iff, Cube.mem_models]
+      constructor
+      · intro h1
+        constructor
+        · intro l hl
+          specialize h1 [l] (by grind)
+          grind
+        · grind
+      · grind
 
 instance {n} : Formula n (Horn n) where
 
@@ -52,24 +107,74 @@ instance {n} : Formula n (Horn n) where
   models := models
 
   models_equiv_right φ M M' h1 := by
-    apply CNF.models_equiv_right
-    intro i hi
-    exact h1 i (φ.subset_vars i hi)
+    simp only [models, CNF.mem_models]
+    intro h2 γ hγ
+    specialize h2 γ hγ
+    rcases h2 with ⟨l, h2, hM⟩
+    have h3 : l.1 ∈ φ.vars.val := by
+      apply φ.subset_vars
+      rw [toCNF] at hγ
+      simp only [Set.mem_union, CNF.mem_vars, Cube.vars]
+      grind
+    specialize h1 l.1 h3
+    simp_all only [Literal.mem_models, eq_iff_iff]
+    use l, h2
+
+def unit_propagate_aux {n} (φ : Horn n) (todo : Cube n) : Horn n :=
+  match todo with
+  | [] => φ
+  | l :: todo =>
+    let res := (φ.clauses.propagate_literal l).partition fun γ ↦ γ.length < 2
+    let empty := res.fst.contains []
+    let todo' := todo ++ res.fst.flatten
+    let φ' := {
+      vars := φ.vars
+      empty := empty
+      unit_literals := l :: φ.unit_literals
+      clauses := res.snd
+      horn_prop := by
+        have h := φ.clauses.IsHorn_propagate_literal (l := l) φ.horn_prop
+        simp only [List.forall_iff_forall_mem] at ⊢ h
+        grind
+      clauses_prop := by
+        simp [res, List.forall_iff_forall_mem]
+      subset_vars := by
+        simp only [Cube.vars, List.mem_cons, exists_eq_or_imp,
+          Set.mem_union, Set.mem_setOf_eq, CNF.mem_vars]
+        intro i hi
+        rcases hi with ⟨rfl | h⟩ | h
+        · sorry
+        · sorry
+        sorry
+    }
+    unit_propagate_aux φ' todo'
+termination_by todo.length + φ.clauses.length
+decreasing_by
+  simp only [List.length_append, add_assoc, List.length_cons,
+    Nat.add_lt_add_iff_left, Nat.lt_one_add_iff]
+  apply Lean.Grind.Nat.le_lo _ _ _ _ (List.length_flatten_short _ (by simp))
+  simp only [List.partition_eq_filter_filter, Function.comp_def, ← List.length_eq_length_filter_add]
+  apply φ.clauses.length_propagate_literal
+
+def unit_propagate {n} (φ : Horn n) :
+  { ψ : Horn n // ψ.unit_literals.vars ∩ ψ.clauses.vars = ∅ } where
+    val := sorry
+    property := sorry
 
 instance {n} : Top n (Horn n) where
 
-  top := Horn.mk VarSet'.empty [] (by simp) (by simp)
+  top := Horn.mk VarSet'.empty false [] [] (by simp) (by simp) (by simp [Cube.vars])
 
   top_correct := by
     ext M
-    simp [Formula.models]
+    simp [Formula.models, models_eq]
 
 instance {n} : Bot n (Horn n) where
 
-  bot := Horn.mk VarSet'.empty [[]] (by simp) (by simp)
+  bot := Horn.mk VarSet'.empty true [] [] (by simp) (by simp) (by simp [Cube.vars])
 
   bot_correct := by
-    simp [Formula.models, models, Formula.vars, Set.ext_iff]
+    simp [Formula.models, models_eq, Formula.vars]
 
 -- Only if this makes ClausalEntailment easier
 instance {n} : Consistency n (Horn n) where
@@ -99,35 +204,44 @@ instance {n} : SententialEntailment n (Horn n) where
 instance {n} : BoundedConjuction n (Horn n) where
 
   and φ ψ :=
-    let formula := φ.formula ++ ψ.formula
-    have h1 : List.Forall Clause.IsHorn formula := by
-      rw [List.forall_append]
-      exact And.intro φ.prop ψ.prop
-    have h2 : ∀ i ∈ formula.vars , i ∈ (φ.vars.union ψ.vars).val := by
-      intro i
-      have := φ.subset_vars i
-      have := ψ.subset_vars i
-      simp_all only [CNF.mem_vars, Prod.exists, VarSet'.mem_union, formula]
-      grind
-    Horn.mk (VarSet'.union φ.vars ψ.vars) formula h1 h2
+    { vars := VarSet'.union φ.vars ψ.vars
+      empty := φ.empty ∨ ψ.empty
+      unit_literals := φ.unit_literals ++ ψ.unit_literals
+      clauses := φ.clauses ++ ψ.clauses
+      horn_prop := by
+        rw [List.forall_append]
+        exact And.intro φ.horn_prop ψ.horn_prop
+      clauses_prop := by
+        rw [List.forall_append]
+        exact And.intro φ.clauses_prop ψ.clauses_prop
+      subset_vars := by
+        intro i
+        have := φ.subset_vars i
+        have := ψ.subset_vars i
+        simp_all only [Cube.vars, Set.mem_union, CNF.mem_vars, List.mem_append, VarSet'.mem_union]
+        grind }
 
   and_correct := by
     intro φ ψ
     ext M
-    simp [Formula.models, Horn.models]
+    simp [Formula.models, models_eq]
     grind
 
 instance {n} : OfPartialModel n (Horn n) where
 
-  ofPartialModel V M := by
-    apply Horn.mk V (CNF.ofPartialModel M)
-    · simp only [List.forall_iff_forall_mem, CNF.ofPartialModel]
-      grind
-    · simp [CNF.ofPartialModel]
-      grind
+  ofPartialModel V M :=
+    { vars := V
+      empty := false
+      unit_literals := Cube.ofPartialModel M
+      clauses := []
+      horn_prop := by simp
+      clauses_prop := by simp
+      subset_vars := by
+        simp [Cube.vars, Cube.ofPartialModel]
+        grind }
 
   ofPartialModel_correct := by
-    simp [instFormula, models]
+    simp [instFormula, models_eq, CNF.models]
 
 instance {n} : Renaming n (Horn n) where
 
@@ -137,9 +251,9 @@ instance {n} : Renaming n (Horn n) where
 
 instance {n} : ToCNF n (Horn n) where
 
-  toCNF := formula
+  toCNF := toCNF
 
-  toCNF_correct := by
-    simp [Formula.models]
+  toCNF_correct φ := by
+    simp only [Formula.models, models]
 
 end Validator.Horn
